monad creation without lists

Test.thy
@@ -1,8 +1,9 @@
 theory Test 
-  imports Main
+  imports Polynomial_Commitment_Schemes
   keywords
   "lift_to_algebraic" :: thy_decl
-begin 
+and  "local_test" :: thy_decl
+begin
 
 ML \<open>
 signature ALGEBRAIC_ALGORITHM =
@@ -12,9 +13,34 @@ val rcodomain_transf : (typ -> typ) -> typ -> typ
 
 val adjoin : typ -> typ -> (typ -> typ)
 
-val lift_to_algebraic : typ -> typ -> typ -> typ
+val lift_to_algebraicT : typ -> typ -> typ -> typ
+
+val strip_spmfT : typ -> typ
+
+val return_spmf : term -> term
 
 val extract_type_params : typ -> string list
+
+val rapply : term list -> term -> term 
+
+val rabs : term list -> term -> term 
+
+(* TODO delete the next two in the interface *)
+val create_names_prod_cases :  Name.context -> typ -> term list * Name.context;
+
+val extract_vec_pair_list: typ -> term list -> term
+
+val constrain_pairs: Name.context -> typ -> typ -> term
+
+val build_ret_term : Name.context -> typ -> term
+
+val abs_typ_over_term : Name.context -> typ -> term -> term
+
+val enforce_alg: Name.context -> term -> term
+
+val build_alg_fun : Name.context -> typ -> term * Name.context
+
+val to_eta_long_term: typ -> term
 
 end;
 
@@ -26,9 +52,174 @@ fun rcodomain_transf f (Type ("fun", [T, U])) = (Type ("fun", [T, f U]))
 
 fun adjoin t vec = fn T => if T = t then Type ("Product_Type.prod", [T, vec]) else T
 
-fun lift_to_algebraic grpT vec = (rcodomain_transf o Term.map_atyps) (adjoin grpT vec)
+fun lift_to_algebraicT grpT vec = (rcodomain_transf o Term.map_atyps) (adjoin grpT vec)
+
+fun strip_spmfT T = T 
+    |> Term.dest_Type_args 
+    |> hd 
+    |> Term.dest_Type_args 
+    |> hd 
+
+fun return_spmf t = 
+  let 
+    val T = Term.fastype_of t 
+  in 
+    \<^Const>\<open>return_pmf \<^Type>\<open>option T\<close> for \<^Const>\<open>Some T for t\<close>\<close>
+  end
 
 fun extract_type_params t = Term.add_tfree_namesT t []
+
+fun rapply [] t = t
+  | rapply (x::xs) t = rapply xs (t $ x) 
+
+fun rabs [] t = t 
+  | rabs (x::xs) t = rabs xs (Term.lambda x t)
+
+fun create_names_prod_cases nctxt  (Type ("Product_Type.prod", [T1, T2])) = 
+    let 
+      val (T2_res,nctxt') = create_names_prod_cases nctxt T2
+      val (T1_res, nctxt'') = create_names_prod_cases nctxt' T1
+    in 
+      (T1_res@T2_res, nctxt'') (*TODO Is this okay?*)
+    end
+  | create_names_prod_cases nctxt T = 
+    let 
+      val (name,nctxt') = Name.variant "" nctxt
+    in 
+      ([Term.Free (name, T)], nctxt') 
+    end;
+
+fun extract_vec_pair_list T (Term.Free(t1N,t1T)::Term.Free(t2N,t2T)::xs) 
+    = if t1T = T andalso t2T = @{typ "int list"} then
+        let 
+          val intlistT =  @{typ "int list"} 
+          val listT = \<^Type>\<open>Product_Type.prod T intlistT\<close>
+          val res = (extract_vec_pair_list T xs)
+          val t1 = Term.Free(t1N,t1T)
+          val t2 = Term.Free(t2N,t2T)
+         in 
+          \<^Const>\<open>List.Cons listT for \<^Const>\<open>Pair T intlistT for t1 t2\<close> res\<close>
+         end
+      else extract_vec_pair_list T xs
+    | extract_vec_pair_list T (_::xs) = extract_vec_pair_list T xs
+    | extract_vec_pair_list T _ =
+      let 
+        val intlistT =  @{typ "int list"} 
+        val listT = \<^Type>\<open>Product_Type.prod T intlistT\<close>
+      in 
+         \<^Const>\<open>list.Nil listT\<close>
+      end
+
+fun constrain_pairs nctxt T resT = resT 
+  |> create_names_prod_cases nctxt 
+  |> fst 
+  |> extract_vec_pair_list T
+  (*TODO here comes the assert*)
+
+fun create_assert T resT = 
+  let 
+    val vlist = constrain_pairs T resT 
+  in 
+    vlist
+  end
+
+(* TODO create a constrain list pairs function. Accordingly create a type lifting that lifts 'g lists
+to a pair ('g list, int list list) 
+This function should also assert that the lists match in size *)
+
+fun build_ret_term_rec nctxt (Type ("Product_Type.prod", [T1, T2])) = 
+  let 
+    val (t2,nctxt') = build_ret_term_rec nctxt T2
+    val (t1,nctxt'') = build_ret_term_rec nctxt' T1
+  in 
+    (\<^Const>\<open>Pair T1 T2 for t1 t2\<close>, nctxt'')
+  end 
+  | build_ret_term_rec nctxt T = 
+  let 
+    val (name,nctxt') = Name.variant "" nctxt
+  in 
+    (Term.Free (name, T), nctxt') 
+  end;
+
+fun build_ret_term nctxt T = 
+   build_ret_term_rec nctxt T |> fst |> return_spmf
+
+fun abs_typ_over_term_rec (Type ("Product_Type.prod", [T1, T2])) (t,nctxt) = 
+  let 
+    val restT = t |> Term.fastype_of (* |> Term.dest_funT |> snd TODO ggf check for fun?*)
+    val (rest,nctxt') = abs_typ_over_term_rec T2 (t,nctxt) |> abs_typ_over_term_rec T1
+  in
+     (\<^Const>\<open>Product_Type.prod.case_prod T1 T2 restT\<close> $ rest, nctxt') (*abs T1 (abs T2)*)
+  end
+  | abs_typ_over_term_rec T (t,nctxt) = 
+  let 
+    val (name,nctxt') = Name.variant "" nctxt
+  in 
+    (Term.absfree (name, T) t, nctxt') 
+  end;
+
+fun abs_typ_over_term nctxt T t = abs_typ_over_term_rec T (t,nctxt) |> fst
+
+fun extract_params nctxt T = 
+  let 
+    val (pramsT, _) = Term.strip_type T;
+    val (pNames,nctxt') = Name.invent' "" (length pramsT) Name.context;
+    val prams = map (fn (n,T) => Term.Free (n, T)) (pNames ~~ pramsT)
+  in 
+    (prams, nctxt') 
+  end
+
+fun supply_prams nctxt t = 
+  let  
+    val T = Term.fastype_of t
+    val (prams,nctxt') = extract_params nctxt T
+  in 
+    (rapply prams t, nctxt')
+  end
+
+fun build_body_term nctxt T = 
+  build_ret_term nctxt T |> abs_typ_over_term nctxt T
+
+fun enforce_alg nctxt t = 
+  let 
+    val (spmf,nctxt') = supply_prams nctxt t
+    val retT = Term.fastype_of spmf |> strip_spmfT
+    val body_term = build_body_term nctxt' retT
+  in 
+     \<^Const>\<open>bind_spmf retT retT for spmf body_term\<close>
+  end
+
+fun build_alg_fun nctxt T = 
+  let
+    (* create params to abstract over*)
+    val (prams,nctxt') = extract_params nctxt T
+    (* instantiate the adversary*)
+    val (advN, nctxt'') = Name.variant "\<A>" nctxt'
+    val adv = Term.Free(advN,T)
+    (* create the fun term to enforce the agm for the adversary *)
+    val fun_term = enforce_alg nctxt adv
+  in 
+    (rabs (rev (adv::prams)) fun_term, nctxt'')
+  end
+
+fun to_eta_long_term t = let 
+  val (pramsT, resT) = Term.strip_type t;
+  val (fName::pNames) = Name.invent Name.context "" (length pramsT+1);
+  val prams = map (fn (n,T) => Term.Free (n, T)) (pNames ~~ pramsT)
+  val alg = Term.Free (fName, t)
+  in
+  rabs (rev (alg::prams)) (rapply prams alg)
+  end
+
+(* TODO write function that takes the free vars list and filters it for group#int_list#xs and 
+  turns it into an Isar level (group*int list) list \<rightarrow> write function that takes the free vars 
+  list, applies the previous described function, and applies create_assert to it.
+
+  Then write a function that takes the free var list and creates prod and abstracts
+
+  Finally put everything together. First create returns spmf, then apply the prod function, then spmf binding. 
+  Once that works, extend with assert.
+*)
 
 end;
 \<close>
@@ -42,28 +233,141 @@ ML \<open>
         val gT = Syntax.read_typ ctxt g;
         val vT = Syntax.read_typ ctxt v;
         val algT = Syntax.read_typ ctxt alg;
-        val agmT = Algebraic_Algorithm.lift_to_algebraic gT vT algT;
+        val agmT = Algebraic_Algorithm.lift_to_algebraicT gT vT algT;
         val tps = Algebraic_Algorithm.extract_type_params agmT;
         val thy' = Sign.add_type_abbrev ctxt (b, tps, agmT) thy
       in thy' end) lthy));
 \<close>
 
-locale semigroup =
-  fixes f :: "'a \<Rightarrow> 'a \<Rightarrow> 'a"
-  assumes assoc: "f (f x y) z = f x (f y z)"
-begin
 
-lemma left_assoc: "f x (f y z) = f (f x y) z"
-  using assoc by simp
+context cyclic_group
+begin 
 
-type_synonym ('g','b', 'a')alg = "'g' \<Rightarrow> 'b' \<Rightarrow> 'a' \<Rightarrow> ('g' * int)"
+fun constrain :: "'a \<Rightarrow> (int list) \<Rightarrow> bool"
+  where "constrain g c_vec = (g = fold (\<lambda>c g. g \<otimes> \<^bold>g [^] c) c_vec \<^bold>g)"
 
-lift_to_algebraic 'g "int list"  "('a,'b,'g)semigroup.alg" => agm_adv
+fun constrain_list :: "('a \<times> int list) list \<Rightarrow> bool"
+  where "constrain_list xs = list_all (\<lambda>(g, c_vec). constrain g c_vec) xs"
 
+type_synonym ('g','b', 'a')alg = "'g' \<Rightarrow> 'b' \<Rightarrow> 'a' \<Rightarrow> ('g' * int*nat) spmf"
+
+lift_to_algebraic 'g "int list"  "('g,'b,'a)cyclic_group.alg" => agm_adv
+
+fun create_assert:: "'x * 'y list \<Rightarrow> bool spmf"
+  where "create_assert (x,y) = return_spmf True"
+
+
+declare [[ML_print_depth = 1000]]
 ML \<open>
-  val t = @{typ "('a,'b,'g)agm_adv"}
+  val agmT = @{typ "('a,'b,'g)agm_adv"}
+
+  val (paramsT, resT) = Term.strip_type agmT
+
+ val boolT = @{typ bool}
+
+ (* val truet = @{term True}
+  
+  val testt = @{term "return_spmf True"}
+
+  (* return_spmf*)
+  val testt' = \<^Const>\<open>return_pmf  \<^Type>\<open>option boolT\<close> for \<^Const>\<open>Some boolT for truet\<close>\<close>*)
+
+  val striped_resT = Algebraic_Algorithm.strip_spmfT resT
+
+  val ret_True = Algebraic_Algorithm.return_spmf @{term True}
+
+  val testgame =  \<^Const>\<open>bind_spmf boolT boolT for ret_True\<close>
+
+  val testgame' = @{term "do {return_spmf True}"}
+
+  val testtt = Algebraic_Algorithm.build_ret_term Name.context striped_resT
+
+  val testttt = Algebraic_Algorithm.abs_typ_over_term Name.context striped_resT testtt 
+
+  val test_term = @{term 
+    "\<lambda>(A::('a,'b,'g)agm_adv) g b a. do { 
+      ((g',c),i,j) \<leftarrow> A g b a;
+      return_spmf ((g',c),i,j) 
+    }"}
+
+ (* val adv_term = Term.Free("A", agmT)
+
+  val test_monad = Algebraic_Algorithm.enforce_alg Name.context adv_term*)
+
+  val test_monad' = Algebraic_Algorithm.build_alg_fun Name.context agmT |> fst
+  
+(*
+ bind_spmf type is not dependent on further statments in the monad, but the monads outcome.
+bind_spmf type is reswspmf \<Rightarrow> (fun resw/ospmf \<Rightarrow> monad res) \<Rightarrow> monad_res 
+
+In terms:
+bind_spmf $ reswspmf $ (fun resw/ospmf \<Rightarrow> monad res)
+
+Product_Type.prod.case_prod typ is:
+(fun newtype \<Rightarrow> function typ) \<Rightarrow> new_type x codomain of fun type \<Rightarrow> domain of fun type
+
+
+Strategy:
+ bind_spmf is just aplly and gives one implicit var for the complete type 
+  \<rightarrow> nothing todo
+  the core is the function that takes the type without spmf and returns the end result type
+  \<rightarrow> here two phases 
+    1. define var decomposition with abs 
+      \<longrightarrow> how to order the names i.e. 
+          create the right names that are used in the body?
+    2. define actual content with the vars. 
+*)
 \<close>
 
+
+ML \<open>
+  Outer_Syntax.local_theory \<^command_keyword>\<open>local_test\<close> "test local definition"
+    (Parse.binding >> (fn b => fn lthy =>
+      let
+        val agmT = @{typ "('a,'b,'g)agm_adv"}
+        val agm_term = Algebraic_Algorithm.to_eta_long_term agmT;
+        val (def, lthy') = Local_Theory.define ((b, NoSyn), ((Thm.def_binding b, []), agm_term)) lthy;
+      in lthy' end));
+\<close>
+
+declare [[show_types]]
+local_test test_adv
+thm test_adv_def 
+
+
 end
+
+
+context abstract_polynomial_commitment_scheme
+begin 
+
+declare [[ML_print_depth = 1000]]
+ML \<open>
+ (*
+   val test2 = @{term "\<lambda>(\<A>::('ck, 'commit, 'state, 'argument, 'evaluation, 'witness) 
+  knowledge_soundness_adversary) (E::('r, 'commit, 'trapdoor) extractor). do {
+  let (\<A>1,\<A>2) = \<A>;
+  (ck,vk) \<leftarrow> key_gen;
+  (c,\<sigma>) \<leftarrow> \<A>1 ck;  
+  (p,d) \<leftarrow> E c;             
+  (i, w) \<leftarrow> \<A>2 \<sigma>;                   
+  let (p_i,_) = w;
+  let (p_i',_) = eval ck d p i;         
+  return_spmf (verify_eval vk c i w \<and> p_i \<noteq> p_i')       
+  }"}
+*)
+
+  val test3 =  @{term eval_bind_game}
+  val test4 =  Term.strip_comb (Thm.prop_of @{thm knowledge_soundness_game_def});
+
+  (*val test3 = Term.strip_abs test2;*)
+
+  (*writeln (Syntax.string_of_term  \<^context> test2);*)
+  (*writeln (@{make_string} test2)*)
+\<close>
+(*TODO find out how c is represented (Var, Abs, Bound, Free, and how to change that)*) 
+
+end
+
 
 end
